\documentclass[../notes.tex]{subfiles}

\pagestyle{main}
\renewcommand{\chaptermark}[1]{\markboth{\chaptername\ \thechapter\ (#1)}{}}
\setcounter{chapter}{2}

\begin{document}




\chapter{Types of Subgroups and Group Functions}
\section{Subgroups and Generators}
\begin{itemize}
    \item \marginnote{10/10:}Defining \textbf{subgroups}.
    \begin{itemize}
        \item Let $G=(G,*)$ be a group, and let $H\subseteq G$ be a subset.
        \item What properties do we want $H$ to satisfy to consider it a "subgroup?"
        \begin{itemize}
            \item $H$ should inherit the binary operation from $G$.
            \item $H$ should be closed under multiplication using said binary operation.
            \item $H$ should be nonempty.
            \item $H$ should contain the inverses of every element --- this is automatic if $G$ is finite since the inverse of an element $g$ of order $n$ is $g^{n-1}$ and $g^{n-1}\in H$ by closure under multiplication.
            \item $H$ should also be associative; we also inherit this for free from $G$.
        \end{itemize}
    \end{itemize}
    \item Easy way to construct a subgroup.
    \begin{itemize}
        \item Let $G$ be a group, and let $x_1,x_2,\dots\in G$. We can let $H=\gen{x_1,x_2,\dots}$, i.e., $H$ is the group \textbf{generated} by $x_1,x_2,\dots$. In other words, $H$ is the set of all finite products $x_1,x_1^{-1},x_2,x_2^{-1},\dots$.
        \item This construction does give you all possible subgroups, but when you write it down, it's very hard to say what group you get.
    \end{itemize}
    \item Example: If you have $H\subset G$ a subgroup, then $H=\gen{h|_{h\in H}}$.
    \item \textbf{Cyclic} (group): A group $G$ for which there exists $g\in G$ such that $G=\gen{g}$.
    \item Examples:
    \begin{itemize}
        \item If $1<n<\infty$, then $\Z/n\Z=\gen{1}$.
        \item However, the generator isn't always unique --- $\Z/7\Z=\gen{3}$.
        \item If $G$ is generated by an element, it's also generated by its inverse. For example, $\Z=\gen{1}=\gen{-1}$.
    \end{itemize}
    \item Proposition: Let $G$ be a cyclic group. It follows that
    \begin{enumerate}
        \item If $|G|=\infty$, then $G$ is isomorphic to $\Z$;
        \item If $|G|=n<\infty$, then $G$ is isomorphic to $\Z/n\Z$.
    \end{enumerate}
    \begin{proof}
        Assertion 1: Let $G=\gen{g}$. Then
        \begin{equation*}
            G = \{\dots,g^{-2},g^{-1},e,g,g^2,g^3,\dots\}
        \end{equation*}
        Now suppose for the sake of contradiction that $g^a=g^b$ for some $a,b\in\Z$. Then $g^{a-b}=e$, so $|G|\leq a-b$, a contradiction. Therefore, $G=\{G^\Z\}$. In particular, we may define $\phi:\Z\to G$ by $k\mapsto g^k$. This map has the property that $a+b\mapsto g^ag^b$, i.e., $\phi(a)\phi(b)=\phi(ab)$\footnote{We all know that this is a \textbf{homomorphism}; Calegari just doesn't want to call it that yet.}.\par
        Assertion 2: Let $G=\gen{g}$. Then
        \begin{equation*}
            G = \{e,g,g^2,\dots,g^{n-1}\}
        \end{equation*}
        Now suppose for the sake of contradiction that $g^a=g^b$. Then $g^{a-b}=e$, so $|G|\leq a-b<n$, a contradiction. Therefore, we may once again define $\phi:\Z/n\Z\to G$ as above. Note that $a+b\mapsto g^{(a+b)\mod n}$. This is still a homomorphism, though.
    \end{proof}
    \item Claim: Any subgroup of a cyclic group is also cyclic.
    \item Example: $G=\Z$, $H=\gen{2002,686}$.
    \begin{itemize}
        \item $H=\{2002x+686y\mid x,y\in\Z\}$.
        \item To say that $H$ is cyclic is to say that it is equal to the integer multiples of some $d\in\Z$, i.e., there exists $d$ such that $G=\{zd\mid z\in\Z\}$.
        \item We can take $d=\gcd(2002,686)$.
        \item (Nonconstructive) proof: Let $d$ be the smallest positive integer in $H$. Suppose for the sake of contradiction that $md+k$ is in the group for some $1\leq k<d$. Then adding $-d$ $m$ times, we get that $k\in H$, a contradiction since we assumed $d$ was the smallest positive integer in $H$.
    \end{itemize}
    \item Let $G=\gen{x,y}$ be a group that is generated by two elements. Find a subgroup $H\subset G$ such that $H$ \emph{must} be generated by more than 2 elements.
    \begin{itemize}
        \item Let's work with $S_n=\gen{(1,2,\dots,n),(1,2)}$.
        \item The subgroup $H=\gen{(1,2),(3,4),(5,6)}$ will work.
        \begin{itemize}
            \item $H=\Z/2\Z\times\Z/2\Z\times\Z/2\Z$.
            \item Suppose $H=\gen{a,b}$. We can get $e,a,b,ab$. But because everything commutes, we can rearrange any product to $a^ib^j$ and cancel.
        \end{itemize}
    \end{itemize}
    \item When you want to answer questions like, "Is $\Z/180180\Z$ a subgroup of $S_n$ for some $n$," you need some more information on the structure of $S_n$.
    \item Group \textbf{presentations} allow us to write and describe a group really easily.
    \begin{itemize}
        \item Seems useful at first, but isn't really that useful once you see it more.
    \end{itemize}
\end{itemize}



\section{Homomorphisms}
\begin{itemize}
    \item \marginnote{10/12:}We've studied groups a lot at this point. But as with vector spaces, we don't have a complete theory of groups until we consider maps between them.
    \item Today: Homomorphisms.
    \item Let $H,G$ be groups.
    \item What qualities do we want a map of groups to have?
    \begin{itemize}
        \item Maps between vector spaces preserve linearity, so maps between groups should probably preserve the group operation.
        \item Bijection? As with linear maps, the bijective case is interesting, but we don't want to be this restrictive.
        \item In fact, that first quality is the only one we want.
    \end{itemize}
    \item \textbf{Homomorphism}: A map $\phi:H\to G$ of sets such that $\phi(x*_Hy)=\phi(x)*_G\phi(y)$.
    \item Lemma: Let $\phi:H\to G$ be a homomorphism. Then\dots
    \begin{enumerate}
        \item $\phi(e_H)=e_G$.
        \item $\phi(x^{-1})=\phi(x)^{-1}$.
    \end{enumerate}
    \begin{proof}
        Claim 1:
        \begin{align*}
            e_G\phi(x) &= \phi(x) = \phi(xe_H) = \phi(x)\phi(e_H)\\
            e_G &= \phi(e_H)
        \end{align*}
        Claim 2:
        \begin{equation*}
            e_G = \phi(e_H) = \phi(xx^{-1}) = \phi(x)\phi(x^{-1})
        \end{equation*}
    \end{proof}
    \item \textbf{Image} (of $\phi$): The subset of $G$ such that for all $h\in H$, $\phi(h)=g$. \emph{Denoted by} $\bm{\im\phi}$.
    \item \textbf{Kernel} (of $\phi$): The subset of $H$ containing all $h\in H$ such that $\phi(h)=e_G$. \emph{Denoted by} $\bm{\ker\phi}$.
    \item Lemma:
    \begin{enumerate}
        \item $\im\phi\subset G$ is a subgroup.
        \item $\ker\phi\subset H$ is a subgroup.
    \end{enumerate}
    \begin{proof}
        % Prove closed under multiplication, inverses, and nonempty. Let $g_1,g_2\in\im\phi$.\par
        % Same idea. Prove...


        Claim 1: We know that $\phi(e_H)=e_G$, so
        \begin{equation*}
            \im\phi \neq \emptyset
        \end{equation*}
        as desired. Next, let $g_1,g_2\in\im\phi$. Suppose $g_1=\phi(h_1)$ and $g_2=\phi(h_2)$. Then since $H$ is closed under multiplication as a subgroup, $h_1h_2\in H$. It follows that
        \begin{equation*}
            g_1g_2 = \phi(h_1)\phi(h_2)
            = \phi(h_1h_2)
            \in \im\phi
        \end{equation*}
        as desired. Lastly, let $g\in\im\phi$. Suppose $g=\phi(h)$. Then since $H$ is closed under inverses as a subgroup, $h^{-1}\in H$. It follows that
        \begin{equation*}
            g^{-1} = \phi(h)^{-1}
            = \phi(h^{-1})
            \in \im\phi
        \end{equation*}
        as desired.\par
        Claim 2: We know that $\phi(e_H)=e_G$, so
        \begin{equation*}
            \ker\phi \neq \emptyset
        \end{equation*}
        as desired. Next, let $g_1,g_2\in\ker\phi$. Then
        \begin{equation*}
            e_G = e_Ge_G
            = \phi(g_1)\phi(g_2)
            = \phi(g_1g_2)
        \end{equation*}
        so $g_1g_2\in\ker\phi$, as desired. Lastly, let $g\in\ker\phi$. Then
        \begin{equation*}
            e_G = \phi(e_H)
            = \phi(gg^{-1})
            = \phi(g)\phi(g^{-1})
            = e_G\phi(g^{-1})
            = \phi(g^{-1})
        \end{equation*}
    \end{proof}
    \item Examples:
    \begin{table}[H]
        \centering
        \small
        \renewcommand{\arraystretch}{1.2}
        \begin{tabular}{c|c|c|c|c}
            $H$ & $G$ & $\phi$ & $\im\phi$ & $\ker\phi$\\
            \hline
            $H$ & $G$ & $\phi(h)=e$ & $\{e\}$ & $H$\\
            $H\leq G$ & $G$ & inclusion & $H$ & $\{e\}$\\
            $\Z$ & $\Z/n\Z$ & $k\mapsto k\mod n$ & $\Z/n\Z$ & $n\Z$\\
            $\text{O}(n)$ & $\R^*$ & $\det$ & $\{\pm 1\}$ & $\text{SO}(n)$\\
            $\text{GL}_n\R$ & $\R^*$ & $\det$ & $\R^*$ & $\text{SL}_n\R$\\
        \end{tabular}
        \caption{Examples of images and kernels.}
        \label{tab:ImKer}
    \end{table}
    \begin{itemize}
        \item The first example shows that there is always at least one homomorphism between two groups.
        \item $\R^*$ is the group of nonzero real numbers with multiplication as the group operation.
        \item The $\text{O}(n)$ example expresses the fact that $\det(AB)=\det(A)\det(B)$, i.e., that the determinant is a homomorphism.
        \begin{itemize}
            \item The kernel is $\text{SO}(n)$ since 1 is the multiplicative identity of $\R^*$ and all matrices in $\text{SO}(n)\subset\text{O}(n)$ get mapped to 1 by the determinant.
        \end{itemize}
        \item $\text{GL}_n\R$ is the set of all $n\times n$ invertible matrices over the field $\R$.
    \end{itemize}
    \item \textbf{Isomorphism}: A bijective homomorphism from $H\to G$.
    \begin{itemize}
        \item If an isomorphism exists between $H$ and $G$, we say, "$H$ is isomorphic to $G$."
    \end{itemize}
    \item Lemma: $H$ is isomorphic to $G$ implies $G$ is isomorphic to $H$.
    \begin{proof}
        $\phi:H\to G$ a bijection implies the existence of $\phi^{-1}:G\to H$. Claim: This is an isomorphism. We can formalize the notion, or just think of $\phi$ as relabeling elements of $H$ and $\phi^{-1}$ as unrelabeling them.
    \end{proof}
    \item Lemma: A homomorphism $\phi:H\to G$ is \textbf{injective} iff $\ker\phi=\{e_H\}$.
    \begin{proof}
        % We will prove that $\ker\phi\neq\{e_H\}$ implies that $\phi$ is not injective, and that $\phi$ is not injective implies $\ker\phi\neq\{e_H\}$.
        % Note that the kernel certainly contains $e_H$ by a previous lemma. Suppose $x\in\ker\phi$ and $x\neq e$. Then $\phi(x)=\phi(e_H)$ so $\phi$ is not injective. Proof by contrapositive here?\par
        % Now assume $\phi$ is not injective. Then $\phi(x)=\phi(y)$ for some $x\neq y$. Let $g=xy^{-1}$. If $g=e$, then $x=y$, a contradiction. Otherwise,
        % \begin{equation*}
        %     \phi(g) = \phi(xy^{-1}) = \phi(x)\phi(y^{-1})
        %     = \phi(x)\phi(y)^{-1}
        %     = \phi(x)\phi(x)^{-1}
        %     = e
        % \end{equation*}
        % Note that we get from the fourth to the fifth entry above using the fact that $\phi(x)=\phi(y)$.

        Suppose $\phi$ is injective. We know that $\phi(e_H)=e_G$ from a previous lemma; this implies that $e_H\in\ker\phi$. Now let $x\in\ker\phi$ be arbitrary. Then $\phi(x)=e_G=\phi(e_H)$. But since $\phi$ is injective, we have that $x=e_H$. Thus, we have proven that $e_H\in\ker\phi$, and any $x\in\ker\phi$ is equal to $e_H$; hence, we know that $\ker\phi=\{e_H\}$, as desired.\par
        Now suppose that $\ker\phi=\{e_H\}$. Let $\phi(x)=\phi(y)$. It follows that
        \begin{equation*}
            \phi(xy^{-1}) = \phi(x)\phi(y^{-1})
            = \phi(x)\phi(y)^{-1}
            = \phi(x)\phi(x)^{-1}
            = e_G
        \end{equation*}
        But this implies that
        \begin{align*}
            xy^{-1} &= e_H\\
            x &= y
        \end{align*}
        as desired.
    \end{proof}
    \item Problem: Is there a surjective homomorphism $\phi:S_5\to S_4$?
    \begin{itemize}
        \item Proposal 1: Send 5-cycles to the identity and everything else to itself.
        \item Proposal 2: "Drop 5" $(1,2)(3,4,5)\mapsto(1,2)(3,4)$.
        \begin{itemize}
            \item Counterexample: $(1,2,3,4,5)\mapsto(1,2,3,4)$.
        \end{itemize}
        \item Proposal 3: If it doesn't do something to everything, send it to $e$.
    \end{itemize}
    \item Lemma: Let $\phi:H\mapsto G$ be a homomorphism. If $|h|=n$, then $|\phi(h)|$ divides $n$, i.e., $n$ is a multiple of $|
    \phi(h)|$.
    \begin{proof}
        If $h^n=e$, then $\phi(h^n)=e=\phi(h)^n$.
    \end{proof}
    \item Equipped with this lemma, let's return to the previous problem.
    \begin{itemize}
        \item Suppose for the sake of contradiction that such a surjective homomorphism $\phi$ exists.
        \item Consider a 5-cycle $h\in S_5$; obviously, $|h|=5$.
        \item It follows by the lemma that $\phi(h)\in S_4$ has order which divides 5. But since the maximum order of an element in $S_4$ is 4, this means that $|\phi(h)|=1$, so $\phi(h)=e$.
    \end{itemize}
    \item If one 5-cycle maps to the identity, then all of their products must, too.
    \item What can map to an order 3 element in $S_4$?
    \item If $\psi(g)=(1,2,3)$, then $|g|$ is divisible by 3.
    \item In fact, no surjective map exists!
    \item In order for homomorphisms to exist, there must be some reason. If there aren't any (nontrivial ones), proving this can be easy.
    \item Now consider $S_4\mapsto S_3$.
    \begin{itemize}
        \item 4-cycles to $e$ or 2-cycles.
        \item 3-cycles to 3-cycles.
    \end{itemize}
    \item Idea: $S_4\cong\text{Cu}\cong S_3$.
    \begin{itemize}
        \item 3 pairs of opposite faces and 4 diagonals.
    \end{itemize}
\end{itemize}



\section{Cosets}
\begin{itemize}
    \item \marginnote{10/14:}Asking, "what's the intuition for this question?" in OH.
    \begin{itemize}
        \item Calegari: Intuition is borne of experience. You get intuition from grubby computations, and then you finally recognize the structure. If you don't know what's going on, it's good to struggle. Start with the simplest possible example and then struggle until you develop intuition.
    \end{itemize}
    \item Last time, we discussed the fact that there is no surjective homomorphism from $S_5\to S_4$, but there is a surjective homomoprhism from $S_4\to S_3$. How about the case $S_{n+1}\to S_n$ for arbitrary $n$?
    \item Teaser theorem: Let $n>m$ and $\phi:S_n\twoheadrightarrow S_m$. Then
    \begin{enumerate}
        \item $m=1$.
        \item $m=2$.
        \item $m=3$.
    \end{enumerate}
    \item Think about the problem of maps from $G\to\Gamma$, where $\Gamma$ is another group. What we know:
    \begin{itemize}
        \item Let $K=\ker\phi$. Recall that $\phi$ is injective iff $\ker\phi=\{e\}$. But there is some additional structure: If $\phi(g)=x$, then $\phi(gK)=x$ where $gK=\{gk\in G\mid k\in K\}$. Another way of phrasing this: If $\phi(g')=x$, then $g'=gk$ for some $k\in K$.
        \item This motivates the following definition.
    \end{itemize}
    \item \textbf{Left coset}: The set defined as follows, where $g\in G$ and $H$ is a subgroup of $G$. \emph{Denoted by} $\bm{gH}$. \emph{Given by}
    \begin{equation*}
        gH = \{gh\mid h\in H\}
    \end{equation*}
    \begin{itemize}
        \item You can define cosets for $H$ a subset (not a subgroup) of $G$, but we will not be interested in these cases.
    \end{itemize}
    \item Claim: $gH\subset G$ means that $gh=gh'$ implies $h=h'$??
    \item Example: $G=S_3$, $H=\gen{e,(1,2)}$.
    \begin{table}[h!]
        \centering
        \small
        \renewcommand{\arraystretch}{1.2}
        \begin{tabular}{c|c}
            $g$ & $gH$\\
            \hline
            $e$ & $\{e,(1,2)\}$\\
            $(1,2)$ & $\{e,(1,2)\}$\\
            $(1,3)$ & $\{(1,3),(1,2,3)\}$\\
            $(1,2,3)$ & $\{(1,3),(1,2,3)\}$\\
            $(2,3)$ & $\{(2,3),(1,3,2)\}$\\
            $(1,3,2)$ & $\{(2,3),(1,3,2)\}$\\
        \end{tabular}
        \caption{Cosets of $\gen{e,(1,2)}$ in $S_3$.}
        \label{tab:S3Cosets}
    \end{table}
    \begin{itemize}
        \item Observations: Cosets are pairwise disjoint. $x\in gH$ implies $xH=gH$.
    \end{itemize}
    \item $\bm{G/H}$: The set of all left cosets of $H$ in $G$.
    \item Proposition:
    \begin{enumerate}
        \item Any two cosets in $G/H$ are either (i) the same or (ii) disjoint.
        \item All $g\in G$ lie in a unique coset (in particular, $gH$).
        \item $|gH|=|H|$.
    \end{enumerate}
    \begin{proof}
        % 2 follows from 1, and 3 from 2 (how??), so we will focus on proving 1.\par
        % Suppose a coset contains $g$. Then it is $gH$. (Argument: If $g\in C_1\cap C_2$, then $C_1=gH$ and $C_2=gH$, so $C_1=C_2$.) Let $C$ a coset contain $g$. Suppose $C=\gamma H$. How do we prove that $gH=\gamma H$? Bidirectional inclusion: If $h\in H$, want $\gamma h\in gH$; if $h\in H$, want to prove there exists $h'\in H$ such that $\gamma h=gh'$. We know that $g\in\gamma H$ implies that there exists $h''$ such that $g=\gamma h''$. We know that $h'=g^{-1}xh=(h'')^{-1}x^{-1}\gamma h=(h'')^{-1}$, $h\in H$. Then $gh=\gamma h''h\in\gamma H$.


        Claim 1: Let $C_1,C_2\in G/H$. We divide into two cases ($C_1\cap C_2=\emptyset$ and $C_1\cap C_2\neq\emptyset$). In the first case, $C_1,C_2$ are disjoint, as desired. In the latter case, they are not disjoint, so we need to prove that they are the same. Suppose $g\in C_1\cap C_2$. Let $C_1=\gamma H$. We will prove that $gH=\gamma H$ via a bidirectional inclusion argument. It will follow by similar logic that $gH=C_2$, from which transitivity will imply that $C_1=gH=C_2$, as desired. Let's begin. Let $x\in gH$. Then $x=gh$ for some $h\in H$. Additionally, we know that $g\in\gamma H$ by hypothesis, so $g=\gamma h'$ for some $h'\in H$. It follows by combining the last two equations that $x=\gamma h'h$. But since $h'h\in H$, $x\in\gamma H$ as desired. A symmetric argument works in the other direction.\par
        Claim 2: We know that $g\in gH$ since $e\in H$ and $g=ge$. Additionally, if $g\in\gamma H$, we have by part (1) that $\gamma H=gH$, so $g$ does lie in a \emph{unique} coset.\par
        Claim 3: Suppose there exist $h,h'\in H$ such that $gh=gh'$. Then $h=h'$ by the cancellation lemma. Thus, every distinct $h\in H$ induces a distinct $gh\in gH$. Therefore, $|gH|=|H|$, as desired.
    \end{proof}
    \item Notice that so far, general statements we've made about groups have been very easy to prove; it's only in particular instances that things become tricky.
    \item Decomposition of a group into equivalence classes: Cosets and conjugacy both do this.
    \item Corollary: Let $H$ be a subgroup of $G$. Then
    \begin{equation*}
        |G| = |G/H|\cdot|H|
    \end{equation*}
    \begin{proof}
        Sketch: Partition $G$ into cosets, each of order $|H|$. But there are $|G/H|$ of these. Thus, the number of elements in $G$ is $|G/H|\cdot|H|$.
    \end{proof}
    \item \textbf{Index} (of $H$ in $G$): The number of cosets into which $H$ partitions $G$. \emph{Denoted by} $\bm{[G:H]}$. \emph{Given by}
    \begin{equation*}
        [G:H] = |G/H|
    \end{equation*}
    \item If $|G|<\infty$, then $[G:H]=|G|/|H|$. If $|G|=\infty$, then we can still define the concept $|G/H|$, but we don't have a nice formula for it.
    \item Example: Let $G=\Z$ and $H=2\Z$ (i.e., $H$ is the set of even integers). Then the orbits are all even and all odd nunbers. The index is 2??
    \item Theorem (Lagrange):
    \begin{enumerate}
        \item Let $G$ be a finite group, $H\subset G$. Then $|H|$ divides $|G|$.
        \item Let $G$ be a finite group. Let $g\in G$. Then $|g|$ divides $|G|$.
    \end{enumerate}
    \item Example: Let $p$ be prime. If $|G|=p$, then $G\cong\Z/p\Z$.
    \begin{proof}
        Take $g\in G$ such that $g\neq e$. By Lagrange's theorem, $|g|$ divides $p$. But this means that $|g|=1$ or $|g|=p$. But it's not the first case because $g\neq e$. Thus, $G=\gen{g}\cong\Z/p\Z$, as desired.
    \end{proof}
    \item \textbf{Right coset}: The set defined as follows, where $g\in G$ and $H$ is a subgroup of $G$. \emph{Denoted by} $\bm{Hg}$. \emph{Given by}
    \begin{equation*}
        Hg = \{hg\mid h\in H\}
    \end{equation*}
    \item $\bm{H/G}$: The set of all right cosets of $H$ in $G$.
    \item The theories of left and right cosets are very similar, but they are not entirely equivalent.
    \begin{itemize}
        \item For example, $H=\gen{e,(1,2)}$ implies
        \begin{align*}
            (1,3)H &= \{(1,3),(1,2,3)\}&
            H(1,3) &= \{(1,3),(1,3,2)\}
        \end{align*}
    \end{itemize}
\end{itemize}




\end{document}